Update project-euler-statements to improve some solver signatures

solvers/100.lean
@@ -29,12 +29,12 @@ example :
   native_decide
 
 
-def solve (_n : Nat) :=
-  (blueRedForTotalLimit (Nat.pow 10 12)).1
+def solve (limit : Nat) :=
+  (blueRedForTotalLimit limit).1
 
-theorem equiv (n : Nat) : ProjectEulerStatements.P100.naive n n = solve n := sorry
+theorem equiv (n : Nat) : ProjectEulerStatements.P100.naive n = solve n := sorry
 end ProjectEulerSolutions.P100
 open ProjectEulerSolutions.P100
 
 def main : IO Unit := do
-  IO.println (solve 0)
+  IO.println (solve (Nat.pow 10 12))
