solvers/18.lean
@@ -35,17 +35,22 @@ abbrev triangle : List (List Nat) := [
   [4, 62, 98, 27, 23, 9, 70, 98, 73, 93, 38, 53, 60, 4, 23]
 ]
 
+def triangleT : ProjectEulerStatements.P18.Triangle 15 := by
+  refine ⟨triangle, ?_⟩
+  decide
+
 
 example : maxPathSum [[3], [7, 4], [2, 4, 6], [8, 5, 9, 3]] = 23 := by
   native_decide
 
 
-def solve (_n : Nat) :=
-  maxPathSum triangle
+def solve {n : Nat} (tri : ProjectEulerStatements.P18.Triangle n) : Nat :=
+  maxPathSum tri.1
 
-theorem equiv (n : Nat) : ProjectEulerStatements.P18.naive = solve n := sorry
+theorem equiv {n : Nat} (tri : ProjectEulerStatements.P18.Triangle n) :
+    ProjectEulerStatements.P18.naive tri = solve tri := sorry
 end ProjectEulerSolutions.P18
 open ProjectEulerSolutions.P18
 
 def main : IO Unit := do
-  IO.println (solve 0)
+  IO.println (solve triangleT)
