solvers/37.lean
@@ -49,8 +49,7 @@ partial def isTruncatablePrime (n : Nat) (isPrime : Array Bool) : Bool :=
         if !isPrime[m]! then false else loopL (k - 1)
     loopR n && loopL (len - 1)
 
-partial def solve : Nat :=
-  let limit := 1000000
+partial def solve (limit : Nat) : Nat :=
   let isPrime := sieve limit
   let rec loop (n found total : Nat) : Nat :=
     if n > limit then
@@ -96,9 +95,9 @@ example :
   native_decide
 
 
-theorem equiv (n : Nat) : ProjectEulerStatements.P37.naive n = solve := sorry
+theorem equiv (n : Nat) : ProjectEulerStatements.P37.naive n = solve n := sorry
 end ProjectEulerSolutions.P37
 open ProjectEulerSolutions.P37
 
 def main : IO Unit := do
-  IO.println solve
+  IO.println (solve 1000000)
