solvers/44.lean
@@ -71,13 +71,12 @@ example : isPentagonal (pentagonal 7 - pentagonal 4) = false := by
   native_decide
 
 
-def solve (_n : Nat) :=
-  findMinDifference 10000
+def solve (limit : Nat) :=
+  findMinDifference limit
 
 theorem equiv (n : Nat) : ProjectEulerStatements.P44.naive n = solve n := sorry
 end ProjectEulerSolutions.P44
 open ProjectEulerSolutions.P44
 
 def main : IO Unit := do
-  let ans := solve 0
-  IO.println ans
+  IO.println (solve 10000)
