solvers/12.lean
@@ -38,7 +38,7 @@ partial def solve (k : Nat) : Nat :=
 example : solve 5 = 28 := by
   native_decide
 
-theorem equiv (n : Nat) : ProjectEulerStatements.P12.naive n n = solve n := sorry
+theorem equiv (n : Nat) : ProjectEulerStatements.P12.naive n = solve n := sorry
 end ProjectEulerSolutions.P12
 open ProjectEulerSolutions.P12
 
